compiler/src/FlatToRiscvDef.v
@@ -9,8 +9,9 @@ Require Import riscv.Decode.
 Require Import riscv.PseudoInstructions.
 Require Import riscv.InstructionCoercions.
 Require Import Coq.micromega.Lia.
+Require Import riscv.AxiomaticRiscv.
 Require Import riscv.Utility.
-
+Require Import riscv.util.ListLib.
 
 Local Open Scope ilist_scope.
 Local Open Scope Z_scope.
@@ -23,6 +24,8 @@ Module Import FlatToRiscvDef.
     LwXLEN: Register -> Register -> Z -> Instruction;
     SwXLEN: Register -> Register -> Z -> Instruction;
     compile_ext_call: list Register -> actname -> list Register -> list Instruction;
+    max_ext_call_code_size: Z;
+    max_ext_call_code_size_nonneg: 0 <= max_ext_call_code_size;
   }.
 End FlatToRiscvDef.
 
@@ -35,6 +38,62 @@ Section FlatToRiscv1.
     Basic_bopnames.funcname := Empty_set;
     Basic_bopnames.actname := actname;
   |}.
+
+  (* Part 1: Definitions needed to state when compilation outputs valid code *)
+
+  Definition stmt_size_body(rec: stmt -> Z)(s: stmt): Z :=
+    match s with
+    | SLoad x a => 1
+    | SStore a v => 1
+    | SLit x v => 8
+    | SOp x op y z => 2
+    | SSet x y => 1
+    | SIf cond bThen bElse => 1 + (rec bThen) + (rec bElse)
+    | SLoop body1 cond body2 => 1 + (rec body1) + (rec body2)
+    | SSeq s1 s2 => 1 + (rec s1) + (rec s2)
+    | SSkip => 1
+    | SCall binds f args => 1 + (Zlength binds + Zlength args)
+    | SInteract binds f args => 1 + (Zlength binds + Zlength args) + max_ext_call_code_size
+    end.
+
+  Fixpoint stmt_size(s: stmt): Z := stmt_size_body stmt_size s.
+  (* TODO: in coq 8.9 it will be possible to state this lemma automatically: https://github.com/coq/coq/blob/91e8dfcd7192065f21273d02374dce299241616f/CHANGES#L16 *)
+  Lemma stmt_size_unfold : forall s, stmt_size s = stmt_size_body stmt_size s. destruct s; reflexivity. Qed.
+
+  Arguments Z.add _ _ : simpl never.
+
+  Lemma stmt_size_pos: forall s, stmt_size s > 0.
+  Proof.
+    induction s; simpl; try omega;
+    pose proof (Zlength_nonneg binds);
+    pose proof (Zlength_nonneg args);
+    pose proof max_ext_call_code_size_nonneg;
+    simpl in *;
+    try omega.
+  Qed.
+
+  (* TODO is 2^9 really the best we can get? *)
+  Definition stmt_not_too_big(s: stmt): Prop := stmt_size s < 2 ^ 9.
+
+  (* This phase assumes that register allocation has already been done on the FlatImp
+     level, and expects the following to hold: *)
+  Fixpoint valid_registers(s: stmt): Prop :=
+    match s with
+    | SLoad x a => valid_register x /\ valid_register a
+    | SStore a x => valid_register a /\ valid_register x
+    | SLit x _ => valid_register x
+    | SOp x _ y z => valid_register x /\ valid_register y /\ valid_register z
+    | SSet x y => valid_register x /\ valid_register y
+    | SIf c s1 s2 => valid_register c /\ valid_registers s1 /\ valid_registers s2
+    | SLoop s1 c s2 => valid_register c /\ valid_registers s1 /\ valid_registers s2
+    | SSeq s1 s2 => valid_registers s1 /\ valid_registers s2
+    | SSkip => True
+    | SCall binds _ args => Forall valid_register binds /\ Forall valid_register args (* untested *)
+    | SInteract binds _ args => Forall valid_register binds /\ Forall valid_register args (* untested *)
+    end.
+
+
+  (* Part 2: compilation *)
 
   Definition compile_op(rd: Register)(op: bopname)(rs1 rs2: Register): list Instruction :=
     match op with
